WIP

src/phl/ecQuantum.ml
@@ -5,6 +5,7 @@ let is_f_glob f =
   | Fglob _ -> true
   | _       -> false
 
+(*
 let is_classical_or_local  =
   let rec is_classical env f =
   match f.f_node with
@@ -23,7 +24,7 @@ let is_classical_or_local  =
   | FequivF _ | FequivS _
   | FeagerF _  | Fcoe _ | Fpr _ -> assert false in
   is_classical
-
+ *)
 
 let rec wf_quantum env f =
   match f.f_node with
@@ -35,12 +36,12 @@ let rec wf_quantum env f =
    (* | Some(`And `Asym), [f1; f2] -> is_classical env f1 && wf_quantum env f2 *)
     | Some(`And `Asym), [f1; f2] -> wf_quantum env f1 && wf_quantum env f2
     | Some(`Or _), [f1; f2] ->
-         is_classical_or_local env f1 && wf_quantum env f2
-      || wf_quantum env f1 && is_classical_or_local env f2
+         is_classical(* _or_local*) env f1 && wf_quantum env f2
+      || wf_quantum env f1 && is_classical (*_or_local*) env f2
     | Some `Imp, [f1; f2] ->
-      is_classical_or_local env f1 && wf_quantum env f2
+      is_classical(*_or_local*) env f1 && wf_quantum env f2
     | Some `Eq, [f1; f2] when is_f_glob f1 && is_f_glob f2 -> true
-    | _ -> is_classical_or_local env f
+    | _ -> is_classical(*_or_local*) env f
     end
   | Fif (f1, f2, f3) ->
     is_classical env f1 && wf_quantum env f2 && wf_quantum env f3
