theories/distributions/DList.ec
@@ -42,34 +42,6 @@ move=> n hn hrec dl.
 by rewrite !foldS //= hrec dmap_dprodR dmap_dprodL !dmap_comp dprodA dmap_comp.
 qed.
 
-lemma dlist01E (d : 'a distr) n x:
-  n <= 0 => mu1 (dlist d n) x = b2r (x = []).
-proof. by move=> /(dlist0 d) ->;rewrite dunit1E (eq_sym x). qed.
-
-lemma dlistS1E (d : 'a distr) x xs:
-  mu1 (dlist d (size (x::xs))) (x::xs) =
-    mu1 d x * mu1 (dlist d (size xs)) xs.
-proof.
-rewrite /= addzC dlistS 1:size_ge0 /= dmap1E -dprod1E &(mu_eq) => z /#.
-qed.
-
-lemma dlist0_ll (d : 'a distr) n:
-  n <= 0 =>
-  is_lossless (dlist d n).
-proof. by move=> /(dlist0 d) ->;apply dunit_ll. qed.
-
-lemma dlist_ll (d : 'a distr) n:
-  is_lossless d =>
-  is_lossless (dlist d n).
-proof.
-move=> d_ll; case (0 <= n); first last.
-+ move=> lt0_n; rewrite dlist0 1:/#;apply dunit_ll.
-elim n=> [|n le0_n ih];first by rewrite dlist0 //;apply dunit_ll.
-by rewrite dlistS //;apply/dmap_ll/dprod_ll.
-qed.
-
-hint exact random : dlist_ll.
-
 lemma supp_dlist0 (d : 'a distr) n xs:
   n <= 0 =>
   xs \in dlist d n <=> xs = [].
@@ -91,6 +63,17 @@ lemma supp_dlist_size (d : 'a distr) n xs:
   0 <= n => xs \in dlist d n => size xs = n.
 proof. by move=> ge0_n; case/(supp_dlist d n xs ge0_n). qed.
 
+lemma dlist01E (d : 'a distr) n x:
+  n <= 0 => mu1 (dlist d n) x = b2r (x = []).
+proof. by move=> /(dlist0 d) ->;rewrite dunit1E (eq_sym x). qed.
+
+lemma dlistS1E (d : 'a distr) x xs:
+  mu1 (dlist d (size (x::xs))) (x::xs) =
+    mu1 d x * mu1 (dlist d (size xs)) xs.
+proof.
+rewrite /= addzC dlistS 1:size_ge0 /= dmap1E -dprod1E &(mu_eq) => z /#.
+qed.
+
 lemma dlist1E (d : 'a distr) n xs:
   0 <= n =>
   mu1 (dlist d n) xs
@@ -103,6 +86,36 @@ move=> le0_n; case (n = size xs)=> [->|].
   by rewrite dlistS1E /= big_cons ih.
 smt w=(supp_dlist mu_bounded).
 qed.
+
+lemma dlist1E_add (d : 'a distr) n1 n2 l : 
+  0 <= n1 => 0 <= n2 =>
+  mu1 (dlist d (n1 + n2)) l = mu1 (dlist d n1) (take n1 l) * mu1 (dlist d n2) (drop n1 l).
+proof.
+  move=> h1 h2.
+  case (size l < n1) => hs. 
+  + rewrite dlist1E 1:/# dlist1E 1://; smt(size_take).
+  rewrite dlist_add //= dmap1E -dprod1E.
+  apply mu_eq_support => -[l1 l2] /= /supp_dprod [] /=.
+  move=> /(supp_dlist_size _ _ _ h1) <<- _.
+  rewrite /(\o) /pred1 /= -{1}(cat_take_drop (size l1) l); smt(eqseq_cat size_take).
+qed.
+
+lemma dlist0_ll (d : 'a distr) n:
+  n <= 0 =>
+  is_lossless (dlist d n).
+proof. by move=> /(dlist0 d) ->;apply dunit_ll. qed.
+
+lemma dlist_ll (d : 'a distr) n:
+  is_lossless d =>
+  is_lossless (dlist d n).
+proof.
+move=> d_ll; case (0 <= n); first last.
++ move=> lt0_n; rewrite dlist0 1:/#;apply dunit_ll.
+elim n=> [|n le0_n ih];first by rewrite dlist0 //;apply dunit_ll.
+by rewrite dlistS //;apply/dmap_ll/dprod_ll.
+qed.
+
+hint exact random : dlist_ll.
 
 lemma dlist0E n (d : 'a distr) P : n <= 0 => mu (dlist d n) P = b2r (P []).
 proof. by move=> le0;rewrite dlist0 // dunitE. qed.
@@ -165,6 +178,13 @@ abstract theory Program.
 
       r <$ dlist d n;
       return r;
+    }
+    proc sample2(n1:int, n2:int) : t list * t * t list = {
+      var rs1,r,rs2;
+      rs1 <$ dlist d n1;
+      r   <$ d;
+      rs2 <$ dlist d n2;
+      return (rs1, r, rs2);
     }
   }.
 
@@ -283,4 +303,50 @@ abstract theory Program.
       by wp; call Sample_Loop_eq.
     by inline *; wp; while (={i, n0} /\ rev l{1} = l{2}); auto; smt.
   qed.
+
+  equiv Sample_Sample2 n1_ n2_ : Sample.sample ~ Sample.sample2 : 
+     n{1} = n1{2} + 1 + n2{2} /\ 0 <= n1{2} /\ 0 <= n2{2} /\ n1{2} = n1_ /\ n2{2} = n2_ ==>
+     res{1} = res{2}.`1 ++ res{2}.`2 :: res{2}.`3 /\
+     size res{2}.`1 = n1_ /\ size res{2}.`3 = n2_.
+  proof.
+    conseq (: _ ==> res{1} = res{2}.`1 ++ res{2}.`2 :: res{2}.`3) _ 
+      (: 0 <= n1 /\ 0 <= n2 /\ n1 = n1_ /\ n2 = n2_ ==> size res.`1 = n1_ /\ size res.`3 = n2_) => //.
+    + by proc; auto; smt(supp_dlist_size).
+    bypr (res{1}) (res{2}.`1 ++ res{2}.`2 :: res{2}.`3) => />.
+    move=> &1 &2 l {n1_ n2_}; move: (arg{1}) (n1{2}) (n2{2}) => /> n1_ n2_ hn1 hn2.
+    have -> : Pr[Sample.sample2(n1_, n2_) @ &2 : res.`1 ++ res.`2 :: res.`3 = l] =
+              mu1 (dlist d (n1_ + 1 + n2_)) l; last first.
+    + by byphoare (: n = n1_ + 1 + n2_ ==> _) => //; proc; rnd (pred1 l); skip.
+    byphoare (: n1 = n1_ /\ n2 = n2_ ==> _) => //; proc.
+    case @[ambient] (size l = n1_ + 1 + n2_) => hs; last first.
+    + conseq (:_ : 0%r); 1: smt(dlist1E).
+      by hoare; auto; smt (supp_dlist size_cat).
+    conseq (: rs1 = take n1_ l /\ r = nth witness l n1_ /\ rs2 = drop (n1_ + 1) l : 
+      = (mu1 (dlist d n1_) (take n1_ l) * 
+          (mu1 d (nth witness l n1_) * mu1 (dlist d n2_) (drop (n1_ + 1) l)))) (: _ ==> size rs1 = n1_ ) => //.
+    + move=> _ _ r rs1 rs2.
+      rewrite -{1 3}(cat_take_drop n1_ l) -(cat_take_drop 1 (drop n1_ l)) -drop_add //. 
+      case: (drop n1_ l) (size_drop n1_ l hn1) => /=; 1: smt().
+      move=> x *; rewrite take0 /= nth_cat size_takel /=; smt (eqseq_cat size_takel).
+    + move=> *; rewrite -addrA (dlist1E_add d _ _ l) // 1:/# dlist1E_add // -drop_add //.
+      do 2!congr; rewrite -{1}(cat_take_drop n1_ l) nth_cat size_takel 1:/# /=.
+      case: (drop n1_ l) (size_drop n1_ l hn1) => /=; 1: smt().
+      by move=> x *; rewrite take0 (dlistS1E d x []) dlist01E.
+    + by auto => /> ? /(supp_dlist_size _ _ _ hn1).
+    seq 1 : (rs1 = take n1_ l) 
+      (mu1 (dlist d n1_) (take n1_ l)) 
+      (mu1 d (nth witness l n1_) * mu1 (dlist d n2_) (drop (n1_ + 1) l))
+      _ 0%r (n2 = n2_) => //.
+    + by conseq />.
+    + by rnd (pred1 (take n1_ l)); skip => />.
+    + conseq />; seq 1 : (r = nth witness l n1_) 
+            (mu1 d (nth witness l n1_)) (mu1 (dlist d n2_) (drop (n1_ + 1) l))
+            _ 0%r (n2 = n2_) => //.
+      + by conseq />.
+      + by rnd (pred1 (nth witness l n1_)).      
+      + by conseq />; rnd (pred1 (drop (n1_ + 1) l)).
+      by conseq (:false) => /> //.
+    by conseq (:false) => /> //.
+  qed. 
+
 end Program.
